templates/hindsight/hindsight.v
@@ -234,37 +234,82 @@ Module HINDSIGHT_DEFS (DS : DATA_STRUCTURE).
     intros _. by apply list_find_None in H'.
   Qed.
 
+  Lemma process_proph_case1_rec tid prf pvs :
+    process_proph tid (prf ++ pvs) = None →
+    Forall (λ x, x.2 ≠ #tid) prf →
+        process_proph tid pvs = None.
+  Proof.
+    intros Hp Hprf. apply process_proph_case1 in Hp. 
+    rewrite /process_proph. destruct (list_find _ pvs) eqn: H'; try done.
+    destruct p as [i x]. apply list_find_Some in H'.
+    apply Forall_app in Hp. destruct Hp as [_ Hp].
+    destruct H' as [H' [H'' _]]. rewrite Forall_lookup in Hp.
+    pose proof Hp i x H' as H1'. by exfalso.
+  Qed.
+
   Lemma process_proph_case2 tid pvs i :
     process_proph tid pvs = Some (i, None) → 
       (∃ x, pvs !! i = Some (x, #tid))
-      ∧ (∀ j, j < i → (pvs !!! j).2 ≠ #tid)
-      ∧ (∀ j, j < i → ¬ (is_snd true (pvs !!! j))).
+      ∧ Forall (λ x, ¬ is_snd true x ∧ x.2 ≠ #tid) (take i pvs).
   Proof.
     rewrite /process_proph. destruct (list_find _ pvs) eqn: H'; try done.
     destruct p as [i' x]. destruct (list_find (is_snd true) _) eqn: H''. 
     { destruct p. try done. }
     intros [=]. subst i'. apply list_find_None in H''. apply list_find_Some in H'.
     destruct x as [x1 x2]. rewrite /= in H'. destruct H' as [Hi [Hx2 Hj]].
-    subst x2. split; last split.
-    - by exists x1.
-    - intros j Hji. assert (is_Some (pvs !! j)) as [[xj1 xj2] Hpvsj]. 
-      { rewrite lookup_lt_is_Some. apply mk_is_Some in Hi. 
-        rewrite lookup_lt_is_Some in Hi. lia. }
-      pose proof Hj j (xj1, xj2) as H'. assert (H1' := Hpvsj).
-      apply list_lookup_total_correct in H1'. rewrite H1'. by apply H'.
-    - intros j Hji. assert (is_Some (pvs !! j)) as [[xj1 xj2] Hpvsj]. 
-      { rewrite lookup_lt_is_Some. apply mk_is_Some in Hi. 
-        rewrite lookup_lt_is_Some in Hi. lia. }
-      rewrite Forall_lookup in H''. pose proof H'' j (xj1, xj2) as H''.
-      rewrite lookup_take in H''; try done. assert (H' := Hpvsj).
-      apply list_lookup_total_correct in H'. rewrite H'. by apply H''.
+    subst x2. split. by exists x1. apply List.Forall_and; try done.
+    rewrite Forall_lookup. apply mk_is_Some, lookup_lt_is_Some in Hi.
+    intros i' x' Hx'. assert (i' < i). apply mk_is_Some, lookup_lt_is_Some in Hx'.
+    rewrite take_length in Hx'. lia.
+    apply (Hj i' x'); try done. rewrite lookup_take in Hx'; try done.
+  Qed.
+
+  Lemma process_proph_case2_rec tid prf pvs i :
+    process_proph tid (prf ++ pvs) = Some(i, None) →
+    Forall (λ x, ¬ is_snd true x ∧ x.2 ≠ #tid) prf →
+        ∃ i', process_proph tid pvs = Some (i', None).
+  Proof.
+    intros Hp Hprf. apply process_proph_case2 in Hp.
+    destruct Hp as [[x Hxtid] Htake]. apply Forall_and in Htake.
+    destruct Htake as [Htake1 Htake2].
+    exists (i - length prf). rewrite /process_proph.
+    assert (prf !! i = None) as Prf_i.
+    { destruct (prf !! i) eqn: H'; try done. exfalso.
+      rewrite (lookup_app_l_Some prf pvs _ _ H') in Hxtid. inversion Hxtid.
+      subst p. rewrite Forall_lookup in Hprf.
+      pose proof Hprf _ _ H' as H''. destruct H'' as [_ H'']. done. }
+    assert (pvs !! (i - length prf) = Some (x, #tid)) as Pvs_i'.
+    { by rewrite lookup_app Prf_i in Hxtid. }
+    destruct (list_find _ pvs) eqn: H'; try done; last first.
+    { exfalso. apply list_find_None in H'. rewrite Forall_lookup in H'.
+      pose proof H' _ _ Pvs_i' as H''. done. }
+    destruct p as [i' x']. apply list_find_Some in H'.
+    destruct H' as (Def_x' & Hx' & Hjtid).
+    assert (i' = i - length prf) as ->.
+    { assert (not (i - length prf < i')).
+      { intros H'. pose proof Hjtid _ _ Pvs_i' H' as H''. done. }
+      assert (not (i' < i - length prf)).
+      { intros H'. assert (i' + length prf < i) as H'' by lia.
+        assert (take i (prf ++ pvs) !! (i' + length prf) = Some x') as H1''.
+        rewrite lookup_take; try done. rewrite lookup_app_r; last by lia.
+        by assert (i' + length prf - length prf = i') as -> by lia.
+        rewrite Forall_lookup in Htake2. pose proof Htake2 _ _ H1'' as H2'. done. }
+      lia. }
+    destruct (list_find _ _) eqn: H'; try done. destruct p as [i' y']. 
+    exfalso. apply list_find_Some in H'. destruct H' as [Hi' [Hy' _]].
+    apply lookup_take_Some in Hi'. destruct Hi' as [Hi' H'].
+    assert (i' + length prf < i) as H'' by lia.
+    assert (take i (prf ++ pvs) !! (i' + length prf) = Some y') as H1''.
+    rewrite lookup_take; try done. rewrite lookup_app_r; last by lia.
+    by assert (i' + length prf - length prf = i') as -> by lia.
+    rewrite Forall_lookup in Htake1. pose proof Htake1 _ _ H1'' as H2'. done. 
   Qed.
 
   Lemma process_proph_case3 tid pvs i j :
-    process_proph tid pvs = Some (i, Some j) → 
-      (∃ x, pvs !! i = Some (x, #tid))
-      ∧ (∀ j', j' < i → (pvs !!! j').2 ≠ #tid)
-      ∧ (j < i) ∧ (is_snd true (pvs !!! j)).
+    process_proph tid pvs = Some (i, Some j) →
+      (j < i) ∧ (∃ x, pvs !! i = Some (x, #tid)) ∧ (is_snd true (pvs !!! j))
+      ∧ Forall (λ x, x.2 ≠ #tid) (take i pvs)
+      ∧ Forall (λ x, ¬ is_snd true x) (take j pvs).
   Proof.
     rewrite /process_proph. destruct (list_find _ pvs) eqn: H'; try done.
     destruct p as [i' x]. destruct (list_find (is_snd true) _) eqn: H''; last done.
@@ -276,17 +321,91 @@ Module HINDSIGHT_DEFS (DS : DATA_STRUCTURE).
       apply mk_is_Some, lookup_lt_is_Some in Hi. rewrite take_length in Hy. lia. }
     assert (is_Some (pvs !! j)) as [[xj1 xj2] Hpvsj]. 
     { rewrite lookup_lt_is_Some. apply mk_is_Some, lookup_lt_is_Some in Hi. lia. }
-    split; last split; last split; try done.
+    split; last split; last split; last split; try done.
     - by exists x1.
-    - intros j' Hji. assert (is_Some (pvs !! j')) as [[xj1' xj2'] Hpvsj']. 
-      { rewrite lookup_lt_is_Some. apply mk_is_Some in Hi. 
-        rewrite lookup_lt_is_Some in Hi. lia. }
-      pose proof Hj j' (xj1', xj2') Hpvsj' Hji as H'.
-      apply list_lookup_total_correct in Hpvsj'. by rewrite Hpvsj'.
     - rewrite lookup_take in Hy; try done. apply list_lookup_total_correct in Hy.
       by rewrite Hy.
+    - rewrite Forall_lookup. intros i' x' Hx'. 
+      assert (i' < i). apply mk_is_Some, lookup_lt_is_Some in Hx'.
+      rewrite take_length in Hx'. lia.
+      apply (Hj i' x'). rewrite lookup_take in Hx'. all: done.
+    - rewrite Forall_lookup. intros i' x' Hx'. 
+      assert (i' < i). apply mk_is_Some, lookup_lt_is_Some in Hx'.
+      rewrite take_length in Hx'. lia.
+      assert (i' < j). apply mk_is_Some, lookup_lt_is_Some in Hx'.
+      rewrite take_length in Hx'. lia.
+      assert (take i pvs !! i' = take j pvs !! i') as H'. 
+      rewrite !lookup_take; try done. rewrite -H' in Hx'.
+      pose proof (Hj' i' x' Hx' H0) as H''. done.
   Qed.
 
-  
+  Lemma process_proph_case3_rec tid prf pvs i j :
+    process_proph tid (prf ++ pvs) = Some(i, Some j) →
+    Forall (λ x, ¬ is_snd true x ∧ x.2 ≠ #tid) prf →
+        ∃ i' j', process_proph tid pvs = Some (i', Some j').
+  Proof.
+    intros Hp Hprf. apply process_proph_case3 in Hp.
+    destruct Hp as [Hji [[x Hxtid] [Hj [Htakei Htakej]]]].
+    rewrite Forall_and in Hprf. destruct Hprf as [Hprf1 Hprf2].
+    exists (i - length prf), (j - length prf). rewrite /process_proph.
+    assert (prf !! i = None) as Prf_i.
+    { destruct (prf !! i) eqn: H'; try done. exfalso.
+      rewrite (lookup_app_l_Some prf pvs _ _ H') in Hxtid. inversion Hxtid.
+      subst p. rewrite Forall_lookup in Hprf2.
+      pose proof Hprf2 _ _ H' as H''. done. }
+    assert (pvs !! (i - length prf) = Some (x, #tid)) as Pvs_i'.
+    { by rewrite lookup_app Prf_i in Hxtid. }
+    assert (prf !! j = None) as Prf_j.
+    { destruct (prf !! j) eqn: H'; try done. exfalso.
+      pose proof (lookup_app_l_Some prf pvs _ _ H') as H''.
+      rewrite Forall_lookup in Hprf1. pose proof Hprf1 _ _ H' as Hprf.
+      rewrite list_lookup_total_alt H'' /= in Hj. done. }
+    assert (is_Some((prf ++ pvs) !! j)) as [y Hy].
+    { rewrite lookup_lt_is_Some. apply mk_is_Some in Hxtid.
+      rewrite lookup_lt_is_Some in Hxtid. lia. }
+    assert ((prf ++ pvs) !! j = pvs !! (j - length prf)) as Pvs_j.
+    { by rewrite lookup_app Prf_j. }
+    destruct (list_find _ pvs) eqn: H'; try done; last first.
+    { exfalso. apply list_find_None in H'. rewrite Forall_lookup in H'.
+      pose proof H' _ _ Pvs_i' as H''. done. }
+    destruct p as [i' x']. apply list_find_Some in H'.
+    destruct H' as (Def_x' & Hx' & Hjtid).
+    assert (i' = i - length prf) as ->.
+    { assert (not (i - length prf < i')).
+      { intros H'. pose proof Hjtid _ _ Pvs_i' H' as H''. done. }
+      assert (not (i' < i - length prf)).
+      { intros H'. assert (i' + length prf < i) as H'' by lia.
+        assert (take i (prf ++ pvs) !! (i' + length prf) = Some x') as H1''.
+        rewrite lookup_take; try done. rewrite lookup_app_r; last by lia.
+        by assert (i' + length prf - length prf = i') as -> by lia.
+        rewrite Forall_lookup in Htakei. pose proof Htakei _ _ H1'' as H2'. done. }
+      lia. }
+    destruct (list_find _ _) eqn: H'; last first.
+    { exfalso. apply list_find_None in H'. rewrite Forall_lookup in H'.
+      assert (take (i - length prf) pvs !! (j - length prf) = Some y) as H''.
+      { rewrite lookup_take. by rewrite lookup_app Prf_j in Hy. 
+        apply lookup_ge_None in Prf_j. lia. }
+      rewrite list_lookup_total_alt Hy /= in Hj.
+      pose proof H' _ _ H'' as H1'. done. }
+    destruct p as [j' y']. repeat apply f_equal.
+    apply list_find_Some in H'. destruct H' as [Hy' [Hy'' Hj'']].
+    assert (not (j' < j - length prf)).
+    { intros H'. assert (j' + length prf < j) as H'' by lia.
+      assert (take j (prf ++ pvs) !! (j' + length prf) = Some y') as H1''.
+      rewrite lookup_take; try done. rewrite lookup_app_r; last by lia.
+      rewrite lookup_take in Hy'; try done.
+      by assert (j' + length prf - length prf = j') as -> by lia. lia.
+      rewrite Forall_lookup in Htakej. pose proof Htakej _ _ H1'' as H2'. done. }
+    assert (not (j - length prf < j')).
+    { intros H'.
+      rewrite list_lookup_total_alt lookup_app Prf_j in Hj.
+      rewrite lookup_app Prf_j in Hy. rewrite Hy /= in Hj.
+      assert (take (i - length prf) pvs !! (j - length prf) = Some y) as H1'.
+      rewrite lookup_take. done. rewrite lookup_ge_None in Prf_i.
+      rewrite lookup_ge_None in Prf_j. clear -Prf_i Prf_j Hji. lia.  
+      pose proof Hj'' _ _ H1' H' as H2'. done. }
+    lia.
+  Qed.
+
   End HINDSIGHT_DEFS.
 
